added merge sort and quick sort with correct extraction

perm.v
@@ -1,7 +1,94 @@
-Require Import Arith.
+Require Import Arith Omega.
 Require Import List. 
 
+Set Implicit Arguments.
+
 Reserved Notation "x '~p' y" (at level 70, no associativity).
+
+Section In.
+
+  Variable (X : Type) (x : X) (eqX_dec : forall y : X, y = x \/ y <> x).
+
+  Theorem In_w_dec l : In x l \/ ~ In x l.
+  Proof.
+    induction l as [ | y l IHl ].
+    + right; red; trivial.
+    + destruct (eqX_dec y); simpl; tauto.
+  Qed.
+
+End In.  
+
+Section add.
+
+    Variable (X : Type) (x : X).
+
+    Implicit Type l : list X.
+
+    Definition add l m := exists l1 l2, m = l1++x::l2 /\ l = l1++l2.
+
+    Fact in_add_0 l : add l (x::l).
+    Proof. exists nil, l; auto. Qed.
+ 
+    Fact in_add_1 y l m : add l m -> add (y::l) (y::m).
+    Proof.
+      intros (l1 & l2 & ? & ?); subst; red.
+      exists (y::l1), l2; auto.
+    Qed.
+
+    Section add_ind.
+
+      Variable P : list X -> list X -> Prop.
+
+      Hypothesis HP0 : forall l, P l (x::l).
+      Hypothesis HP1 : forall y l m, P l m -> P (y::l) (y::m).
+
+      Theorem add_ind : forall l m, add l m -> P l m.
+      Proof.
+        intros l m (l1 & l2 & ? & ?); subst.
+        induction l1 as [ | y l1 IH ].
+        + apply HP0.
+        + simpl; apply HP1, IH.
+      Qed.
+  
+    End add_ind.
+
+    Fact add_nil_inv l : add l nil -> False.
+    Proof.
+      intros ([|] & ? & ? & _); discriminate.
+    Qed.
+
+    Fact add_cons_inv l y m : add l (y::m) -> x = y /\ l = m 
+                                           \/ exists l', l = y::l' /\ add l' m.
+    Proof.
+      intros ([ | u l1 ] & l2 & H1 & H2); simpl in *; inversion H1; subst; auto.
+      right; exists (l1++l2); split; auto.
+      exists l1, l2; auto.
+    Qed.
+
+End add.
+
+Hint Resolve in_add_0 in_add_1.
+
+Section split.
+
+  Variable (X : Type) (x y : X).
+
+  Fact split_inv l1 r1 l2 r2 : l1++x::r1 = l2++y::r2 
+                            -> (exists m, l1 = l2++y::m /\ r2 = m++x::r1)  
+                            \/ l1 = l2 /\ x = y /\ r1 = r2
+                            \/ (exists m, l2 = l1++x::m /\ r1 = m++y::r2).
+  Proof.
+    revert l2.
+    induction l1 as [ | u l1 IH ]; intros [ | v l2 ]; simpl; inversion 1; auto.
+    + do 2 right; exists l2; auto.
+    + left; exists l1; auto.
+    + destruct (IH _ H2) as [ (m & ? & ?) | [ (? & ? & ?) | (m & ? & ?) ] ]; subst.
+      - left; exists m; auto.
+      - right; left; auto.
+      - do 2 right; exists m; auto.
+  Qed.
+
+End split.
 
 Section perm.
 
@@ -21,20 +108,15 @@ Section perm.
                                ->      l1 ~p l3
 
   where "x '~p' y " := (perm x y).
+  
+  Hint Constructors perm.
 
   Fact perm_refl l : l ~p l.
   Proof.
-  Admitted.
-
-  Fact perm_length l1 l2 : l1 ~p l2 -> length l1 = length l2.
-  Proof.
-    intros H.
-    induction H as [ 
-                   | x l1 l2 H1 IH1 
-                   | x y l 
-                   | l1 l2 l3 H1 IH1 H2 IH2 
-                   ].
-  Admitted.
+    induction l as [ | x l IH ].
+    + apply perm_nil.
+    + apply perm_cons, IH.
+  Qed.
 
   Fact perm_sym l1 l2 : l1 ~p l2 -> l2 ~p l1.
   Proof.
@@ -43,19 +125,45 @@ Section perm.
                    | x l1 l2 H1 IH1 
                    | x y l 
                    | l1 l2 l3 H1 IH1 H2 IH2 
-                   ].
-  Admitted.
+                   ]; auto.
+    apply perm_trans with (1 := IH2); trivial.
+  Qed.
+
+  Fact perm_length l1 l2 : l1 ~p l2 -> length l1 = length l2.
+  Proof.
+    intros H.
+    induction H as [ 
+                   | x l1 l2 H1 IH1 
+                   | x y l 
+                   | l1 l2 l3 H1 IH1 H2 IH2 
+                   ]; simpl; trivial.
+    f_equal; trivial.
+    rewrite IH1; trivial.
+  Qed.
 
   Fact perm_middle x l r : x::l++r ~p l++x::r.
   Proof.
     induction l as [ | y l IHl ]; simpl.
-  Admitted.
+    + apply perm_refl.
+    + apply perm_trans with (1 := perm_swap _ _ _); auto.
+  Qed.
 
-  Let perm_app_l l r1 r2 : r1 ~p r2 -> l++r1 ~p l++r2.
+  Fact perm_special x k l r : k ~p l++r -> x::k ~p l++x::r.
   Proof.
-    intros;
-    induction l as [ | z l IHl ].
-  Admitted.
+    intros H; apply perm_trans with (2 := perm_middle _ _ _), perm_cons, H.
+  Qed.
+
+  Fact perm_app_comm l m : l ++ m ~p m ++ l.
+  Proof.
+    induction l; simpl.
+    * rewrite <- app_nil_end; apply perm_refl.
+    * apply perm_special; trivial.
+  Qed.
+
+  Fact perm_app_l l r1 r2 : r1 ~p r2 -> l++r1 ~p l++r2.
+  Proof.
+    intros; induction l; simpl; auto.
+  Qed.
 
   Fact perm_app l1 l2 r1 r2 : l1 ~p l2 -> r1 ~p r2 -> l1++r1 ~p l2++r2.
   Proof.
@@ -65,22 +173,189 @@ Section perm.
                    | x y l 
                    | l1 l2 l3 H1 IH1 H2 IH2 
                    ]; intros r1 r2 H12; simpl; auto.
-  Admitted.
+     apply perm_trans with (1 := perm_swap _ _ _), perm_app_l with (l := _::_::_); auto.
+     apply perm_trans with (1 := IH1 _ _ H12), IH2, perm_refl.
+  Qed.
 
   (* incl is defined in the List module of the Standard library *)
 
   Print incl.
-  SearchAbout [ incl ].
 
   Fact perm_incl l m : l ~p m -> incl l m.
   Proof.
     intros H.
-    induction H as [ | x l1 l2 H1 IH1 | x y l | l1 l2 l3 H1 IH1 H2 IH2 ]; simpl; auto.
-  Admitted. 
+    induction H as [ | x l1 l2 H1 IH1 | x y l | l1 l2 l3 H1 IH1 H2 IH2 ]; red; simpl; auto.
+    + intros a [ ? | H ]; subst; auto.
+    + intros a [ ? | [ ? | H ] ]; subst; auto.
+  Qed.
+
+  Fact perm_equal x y : x::nil ~p y::nil -> x = y.
+  Proof.
+    intros H.
+    apply perm_incl in H.
+    specialize (H x); simpl in H.
+    destruct H as [ ? | [] ]; subst; auto.
+  Qed.
+
+  Hint Resolve perm_refl.
+
+  Fact add_perm x l m : add x l m -> x::l ~p m.
+  Proof. intros (? & ? & ? & ?); subst; apply perm_middle. Qed.
+
+  Fact add_perm_rev x l m : add x l m -> m ~p x::l.
+  Proof. intro; apply perm_sym, add_perm; trivial. Qed.
+
+  Fact add_perm' x l m : add x l (x::m) -> l ~p m.
+  Proof.
+    intros ([|] & ? & H1 & H2); subst; inversion H1; subst; auto; apply perm_middle. 
+  Qed.
+
+  Fact add_perm_rev' x l m : add x l (x::m) -> m ~p l.
+  Proof. intro; apply perm_sym, add_perm' with x; trivial. Qed.
+
+  Hint Resolve add_perm add_perm_rev add_perm' add_perm_rev'.
+  
+  Fact add_perm_inv x l1 m1 m2 : m1 ~p m2 -> add x l1 m1 -> exists l2, l1 ~p l2 /\ add x l2 m2.
+  Proof.
+    intros H; revert H x l1. 
+    induction 1 as [ 
+                   | x l1 l2 H1 IH1 
+                   | x y l 
+                   | l1 l2 l3 H1 IH1 H2 IH2 
+                   ]; intros u l' H.
+    + apply add_nil_inv in H; tauto.
+    + apply add_cons_inv in H.
+      destruct H as [ (? & ?) | (l3 & ? & H3) ]; subst.
+      * exists l2; auto.
+      * apply IH1 in H3.
+        destruct H3 as (l4 & H3 & H4).
+        exists (x::l4); auto.
+    + apply add_cons_inv in H.
+      destruct H as  [ (? & ?) | (l1 & ? & H) ]; subst.
+      * exists (y::l); auto.
+      * apply add_cons_inv in H.
+        destruct H as  [ (? & ?) | (l2 & ? & H) ]; subst.
+        - exists (x::l); auto.
+        - exists (y::x::l2); auto.
+    + apply IH1 in H.
+      destruct H as (l4 & G1 & H).
+      apply IH2 in H.
+      destruct H as (l5 & G2 & H).
+      exists l5; split; auto.
+      apply perm_trans with (1 := G1); auto.
+  Qed.
+
+  Fact perm_add_inv ll mm : ll ~p mm -> forall x l m, add x l ll -> add x m mm -> l ~p m.  
+  Proof.
+    induction 1 as [ 
+                   | x l1 l2 H1 IH1 
+                   | x y l 
+                   | l1 l2 l3 H1 IH1 H2 IH2 
+                   ]; intros z u v H3 H4.
+    + apply add_nil_inv in H3; tauto.
+    + apply add_cons_inv in H3;
+      apply add_cons_inv in H4.
+      destruct H3 as [ (? & ?) | (l' & ? & H3) ]; 
+      destruct H4 as [ (? & ?) | (m' & ? & H4) ]; subst; auto.
+      * apply perm_trans with (1 := H1); auto.
+      * apply perm_trans with (2 := H1); auto.
+      * apply perm_cons, IH1 with z; auto.
+    + apply add_cons_inv in H3;
+      apply add_cons_inv in H4.
+      destruct H3 as [ (? & ?) | (l' & ? & H3) ]; 
+      destruct H4 as [ (? & ?) | (m' & ? & H4) ]; subst; auto.
+      * apply perm_cons, add_perm_rev' with x; auto.
+      * apply perm_cons, add_perm' with y; auto.
+      * apply add_cons_inv in H3;
+        apply add_cons_inv in H4.
+        destruct H3 as [ (? & ?) | (l'' & ? & H3) ]; 
+        destruct H4 as [ (? & ?) | (m'' & ? & H4) ]; subst; auto.
+        - apply perm_trans with (1 := perm_swap _ _ _).
+          do 2 apply perm_cons.
+          destruct H3 as (l1 & l2 & ? & ?);
+          destruct H4 as (m1 & m2 & ? & ?); subst.
+          apply split_inv in H1.
+          destruct H1 as [ (m & ? & ?) | [ (? & ? & ?) | (m & ? & ?) ] ]; subst; auto.
+          ** rewrite app_ass; simpl; apply perm_app; auto; apply perm_middle.
+          ** rewrite app_ass; simpl; apply perm_app; auto; apply perm_sym, perm_middle.
+    + apply add_perm_inv with (1 := H1) in H3.
+      destruct H3 as (w & H3 & H5).
+      apply perm_trans with (1 := H3).
+      apply IH2 with z; auto.
+  Qed.
+
+  Fact perm_cons_inv x l m : x::l ~p x::m -> l ~p m.
+  Proof. intro; apply perm_add_inv with (x::l) (x::m) x; auto. Qed.
+
+  Hint Resolve perm_cons_inv.
+
+  Fact perm_app_inv l m k : l++m ~p l++k -> m ~p k.
+  Proof.
+    intro H; induction l; simpl; auto.
+    apply perm_cons_inv in H; auto.
+  Qed.
+  
+  Fact perm_app_perm_inv l1 l2 r1 r2 : l1 ~p l2 -> l1++r1 ~p l2++r2 -> r1 ~p r2.
+  Proof.
+    intros H1 H2.  
+    apply perm_app_inv with l2, perm_trans with (2 := H2), perm_sym.
+    do 2 apply perm_sym, perm_trans with (1 := perm_app_comm _ _).
+    apply perm_app_l; auto.
+  Qed.
+
+  Section perm_dec.
+ 
+    Let perm_dec_1 : (forall l m, l ~p m \/ ~ l ~p m) -> (forall x y : X, x = y \/ x <> y).
+    Proof.
+      intros H x y.
+      destruct (H (x::nil) (y::nil)) as [ H1 | H1 ].
+      + left; revert H1; apply perm_equal.
+      + right; contradict H1; subst; auto.
+    Qed.
+
+    Let perm_dec_2 : (forall x y : X, x = y \/ x <> y) -> (forall l m, l ~p m \/ ~ l ~p m).
+    Proof.
+      intros H.
+      induction l as [ | x l IH ]; intros [ | y m ].
+      + left; auto.
+      + right; intros C; apply perm_length in C; discriminate.
+      + right; intros C; apply perm_length in C; discriminate.
+      + destruct (@In_w_dec _ x) with (l := m) as [ G1 | G1 ].
+        - intro; auto.
+        - apply in_split in G1.
+          destruct G1 as (m1 & m2 & ?); subst.
+          destruct (IH (y::m1++m2)) as [ G1 | G1 ].
+          * left; apply perm_special with (l := _::_); auto.
+          * right; contradict G1.
+            apply perm_cons_inv with x, 
+                  perm_trans with (1 := G1),
+                  perm_trans with (2 := perm_swap _ _ _),
+                  perm_cons, perm_sym, perm_middle.
+        - destruct (H x y) as [ E | D ].
+          * subst.
+            destruct (IH m) as [ H1 | H1 ].
+            ++ left; auto.
+            ++ right; contradict H1.
+               revert H1; apply perm_cons_inv.
+          * right; contradict G1.
+            apply perm_incl in G1.
+            destruct (G1 x) as [ G2 | G2 ]; simpl; subst; tauto.
+    Qed.
+
+    Theorem perm_dec : (forall x y : X, x = y \/ x <> y) 
+                   <-> (forall l m, l ~p m \/ ~ l ~p m).
+    Proof. split; auto. Qed.
+
+  End perm_dec.
 
 End perm.
 
-Infix "~p" := (perm _).
+Infix "~p" := (@perm _).
+
+Hint Constructors perm.
+Hint Resolve perm_special perm_refl perm_app.
+
+Check perm_dec.
 
     
 
