quicksort.v
@@ -1,18 +1,14 @@
-Require Import Arith.
-Require Import List.
-Require Import Bool.
+Require Import Arith List Bool Omega Extraction.
 
-Require Import list_utils.
-Require Import perm.
-Require Import sorted.
+Require Import list_utils perm sorted.
 
 Section quicksort.
 
   Fixpoint pivot x m :=
     match m with 
-      | nil  => (nil,nil)
-      | y::m => let (l,r) := pivot x m
-                in if y <b x then (y::l,r) else (l,y::r)
+      | nil   => (nil,nil)
+      | y::m' => let (l,r) := pivot x m'
+                 in if y <b x then (y::l,r) else (l,y::r)
     end.
 
   Proposition pivot_spec x m : let (l,r) := pivot x m 
@@ -20,72 +16,156 @@ Section quicksort.
                                /\ ub l x = true
                                /\ lb r (S x) = true.
   Proof.
-    induction m as [ | y m IHm ]; simpl.
-
-    repeat split; auto.
-    apply perm_nil.
-
+    induction m as [ | y m IHm ]; simpl; auto.
     destruct (pivot x m) as (l,r).
     destruct IHm as (H1 & H2 & H3).
     case_eq (y <b x); intros H.
-  Admitted.
+    + split; simpl; auto.
+      split; auto.
+      apply andb_true_iff; split; auto.
+    + split; auto.
+      split; auto.
+      destruct y as [ | y ]; simpl.
+      * apply Nat.leb_nle in H; omega.
+      * apply andb_true_iff; split; auto.
+        apply Nat.leb_le.
+        apply Nat.leb_nle in H; omega.
+  Qed.
+
+  Let pivot_type x m (piv : list nat * list nat) := let (l,r) := piv in m ~p l++r /\ ub l x = true /\ lb r x = true.
     
-  Proposition pivot_prop x m : let (l,r) := pivot x m 
-                               in m ~p l++r 
-                               /\ ub l x = true
-                               /\ lb r x = true.
+  Proposition pivot_prop x m : pivot_type x m (pivot x m).
   Proof.
     generalize (pivot_spec x m).
     destruct (pivot x m) as (l,r).
-    intros ( ? & ? & ? ); repeat split; auto.
-    revert H1; apply lb_inc.
-    apply le_bool_le.
-    auto.
+    intros (? & ? & ?); repeat split; auto.
+    revert H1; apply lb_inc, le_bool_le; auto.
   Qed.
+
+  Section qs.
+
+    Inductive qs_graph : list nat -> list nat -> Prop :=
+      | in_qsg_0 : qs_graph nil nil
+      | in_qsg_1 : forall x m l r, qs_graph (fst (pivot x m)) l
+                                -> qs_graph (snd (pivot x m)) r
+                                -> qs_graph (x::m) (l++x::r).
+
+    Let qs_rec m : sig (qs_graph m).
+    Proof.
+      induction m as [ m IH ] using (measure_rect _ (@length _)); revert IH.
+      refine  (match m with 
+        | nil  => fun IH =>       exist _ nil _
+        | x::m => fun IH => 
+        match pivot x m as piv return pivot x m = piv -> _ with
+          | (l,r) => fun E => let (l',G1) := IH l _ in
+                              let (r',G3) := IH r _ 
+                              in  exist _ (l'++x::r') _
+        end eq_refl
+      end); try (constructor; fail); generalize (pivot_prop x m); rewrite E.
+      + intros (H & _); apply perm_length in H; simpl; rewrite H, app_length; omega.
+      + intros (H & _); apply perm_length in H; simpl; rewrite H, app_length; omega.
+      + intros (H1 & H2 & H3); constructor; rewrite E; simpl; auto.
+    Qed.
+
+    Definition qs m := proj1_sig (qs_rec m).
+
+    Fact qs_spec m : qs_graph m (qs m).
+    Proof. apply (proj2_sig _). Qed.
+
+    Fact qs_correct m : m ~p qs m /\ sorted (qs m).
+    Proof.
+      generalize (qs m) (qs_spec m).
+      induction 1 as [ | x m l' r' H1 (G1 & G2) H2 (G3 & G4) ]; auto.
+      generalize (pivot_prop x m); destruct (pivot x m) as (l,r); simpl in *.
+      intros (H3 & H4 & H5); split.
+      + apply perm_special, perm_trans with (1 := H3); auto.
+      + apply quick_sorted; auto.
+        * revert H4; apply ub_incl, perm_incl, perm_sym; auto.
+        * revert H5; apply lb_incl, perm_incl, perm_sym; auto.
+    Qed.
+
+  End qs.
+
+  Definition quicksort m : { k | m ~p k /\ sorted k }.
+  Proof.
+    induction m as [ m IH ] using (measure_rect _ (@length _)); revert IH.
+    refine (match m with 
+      | nil  => fun IH =>       exist _ nil _
+      | x::m => fun IH => 
+      match pivot x m as piv return pivot_type x m piv -> _ with
+        | (l,r) => fun H => let (l',G1) := IH l _ in
+                            let (r',G3) := IH r _ 
+                            in  exist _ (l'++x::r') _
+
+      end (pivot_prop x m)
+    end).
+    1,2,3 : cycle 1.
+
+    (* Termination certificates *)
+
+    + apply proj1, perm_length in H; simpl; rewrite H, app_length; omega.
+    + apply proj1, perm_length in H; simpl; rewrite H, app_length; omega.
+
+    (* Post-conditions *)
+
+    + split; auto; constructor.
+    + destruct H as (H1 & H2 & H3).
+      destruct G1 as (G1 & G2).
+      destruct G3 as (G3 & G4). 
+      split.
+      - apply perm_special, perm_trans with (1 := H1); auto.
+      - apply quick_sorted; auto.
+        * revert H2; apply ub_incl, perm_incl, perm_sym; auto.
+        * revert H3; apply lb_incl, perm_incl, perm_sym; auto.
+  Defined.
 
   (* quick_sort_rec : by induction on the length n of the list m *)
 
-  Fixpoint quick_sort_rec n m := 
+  Definition quick_sort_rec : nat -> list nat -> list nat := fix loop n m := 
     match n, m with 
       | O  , _    => nil
       | S n, nil  => nil
       | S n, x::m => let (l,r) := pivot x m
-                     in  (quick_sort_rec n l)++x::(quick_sort_rec n r)
+                     in  (loop n l)++x::(loop n r)
     end.
 
   (* assuming m has length lower than n, then it is correctly sorted by quick_sort_rec 
      ie quick_sort_rec n m is a permutation of m which is sorted 
   *)
 
-  Proposition quick_sort_rec_prop n : forall m, length m < n -> m ~p quick_sort_rec n m 
-                                                             /\ sorted (quick_sort_rec n m).
+  Proposition quick_sort_rec_prop n m : length m <= n -> m ~p quick_sort_rec n m /\ sorted (quick_sort_rec n m).
   Proof.
-    induction n as [ | n IHn ]; intros [ | x m ] Hm; simpl; auto; simpl in Hm;
-    try (apply lt_n_O in Hm; elim Hm).
-
-    split; auto.
-    apply perm_nil.
-
-    generalize (pivot_prop x m).
-    destruct (pivot x m) as (l,r).
-    intros ( H1 & H2 & H3 ).
-    apply lt_S_n in Hm.
-
-    destruct (IHn l) as (H4 & H5).
- 
-  Admitted.
+    revert n; induction m as [ [ | x m ] IHm ] using (measure_rect _ (@length _)). 
+    + destruct n; simpl; split; auto.
+    + intros [ | n ] Hn; simpl in Hn |- *; try omega.
+      generalize (pivot_prop x m).
+      destruct (pivot x m) as (l,r).
+      intros (H1 & H2 & H3).
+      generalize (perm_length H1); rewrite app_length; intros H4.
+      destruct (IHm l) with (n := n) as (H5 & H6); try (simpl; omega).
+      destruct (IHm r) with (n := n) as (H7 & H8); try (simpl; omega).
+      split; auto.
+      * apply perm_special, perm_trans with (1 := H1), perm_app; auto.
+      * apply quick_sorted; auto; 
+          [ revert H2; apply ub_incl | revert H3; apply lb_incl ]; 
+          apply perm_incl, perm_sym; auto.
+  Qed.
 
   (* compute the length of m before calling quick_sort_rec *)
  
   Definition quick_sort m := quick_sort_rec (S (length m)) m.
 
   Proposition quick_sort_prop m : m ~p quick_sort m /\ sorted (quick_sort m).
-  Proof.
-    apply quick_sort_rec_prop.
-    auto.
-  Qed.
+  Proof. apply quick_sort_rec_prop; auto. Qed.
 
 End quicksort.
+
+Extraction Inline quick_sort_rec.
+
+Recursive Extraction quicksort quick_sort qs.
+
+Check qs_correct.
+Check quicksort.
 
 Eval compute in quick_sort (2::3::1::8::1::10::3::5::2::nil).
 
