list_utils.v
@@ -1,4 +1,4 @@
-Require Import List.
+Require Import List Omega Wellfounded Extraction.
 
 Definition app_split { X : Type } (l1 l2 r1 r2 : list X) : 
    l1++r1 = l2++r2 -> (exists m, l2 = l1++m /\ r1 = m++r2) 
@@ -15,3 +15,41 @@ Proof.
   left; exists m; subst; auto.
   right; exists m; subst; auto.
 Qed.
+
+Section measure_ind.
+
+  Variable (X : Type) (m : X -> nat) (P : X -> Type)
+           (HP : forall x, (forall y, m y < m x -> P y) -> P x).
+
+  Let R x y := m x < m y.
+
+  Theorem measure_rect x : P x.
+  Proof.
+    cut (Acc R x).
+    + revert x.
+      exact (fix loop x Hx { struct Hx } := HP x (fun y Hy => loop y (Acc_inv Hx Hy))).
+    + unfold R; apply wf_inverse_image, lt_wf.
+  Qed.
+
+End measure_ind.
+
+Section measure_double_ind.
+
+  Variable (X Y : Type) (m : X -> Y -> nat) (P : X -> Y -> Type)
+           (HP : forall x y, (forall x' y', m x' y' < m x y -> P x' y') -> P x y).
+
+  Let R c d := m (fst c) (snd c) < m (fst d) (snd d).
+
+  Theorem measure_double_rect x y : P x y.
+  Proof.
+    cut (Acc R (x,y)).
+    + revert x y.
+      refine (fix loop x y H { struct H } := HP x y (fun x' y' H' => loop x' y' (Acc_inv H _))).
+      apply H'.
+    + unfold R; apply wf_inverse_image, lt_wf.
+  Qed.
+
+End measure_double_ind.
+
+Extraction Inline measure_double_rect.
+Extraction Inline measure_rect.
