merge_sort.v
@@ -1,0 +1,117 @@
+Require Import Arith List Omega.
+
+Require Import list_utils perm sorted.
+
+Section mergesort.
+
+  Section merge.
+
+    Let merge_perm_1 (x y : nat) l m k : k ~p l++y::m -> x::k ~p x::l++y::m.
+    Proof. intro; auto. Qed.
+
+    Let merge_perm_2 (x y : nat) l m k : k ~p x::l++m -> y::k ~p x::l++y::m.
+    Proof.
+      intros H. 
+      apply perm_special with (l := x::l),
+            perm_trans with (1 := H), perm_refl. 
+    Qed.
+
+    Let merge_le_bool x y : x <b y = false -> y <b x = true.
+    Proof. intros H; apply Nat.leb_le; apply Nat.leb_nle in H; omega. Qed.
+
+    Let merge_sorted x y l m k : x <b y = true 
+                              -> sorted (x::l) 
+                              -> sorted (y::m) 
+                              -> sorted k 
+                              -> k ~p l++y::m 
+                              -> sorted (x::k).
+    Proof.
+      intros H1 H2 H3 H4 H5.
+      apply sorted_cons; split; auto.
+      apply lb_incl with (l++y::m).
+      * apply perm_incl; auto.
+      * rewrite lb_app.
+        apply sorted_inv_lb in H2.
+        apply sorted_inv_lb in H3.
+        apply andb_true_intro; split; auto.
+        simpl; apply andb_true_intro; split; auto.
+        revert H3; apply lb_inc; auto.
+    Qed.
+
+    Definition merge l m : sorted l -> sorted m -> { k | k ~p l++m /\ sorted k }.
+    Proof.
+      pattern l, m; revert l m; apply measure_double_rect with (m := fun x y => length x+length y).
+      intros l m IH Hl Hm.
+      case_eq l.
+      + exists m; subst; split; auto; apply perm_refl.
+      + intros x l' H1.
+        case_eq m.
+        * intros H2; exists l; split; auto.
+          rewrite <- H1, <- app_nil_end; apply perm_refl.
+        * intros y m' H2.
+          case_eq (x <b y); intros H3; [ | apply merge_le_bool in H3 ].
+          - refine (let (k,G) := IH l' m _ _ _ in _); auto; try destruct G as (G1 & G2).
+            ++ subst; simpl; omega.
+            ++ revert Hl; subst; apply sorted_inv_sorted.
+            ++ exists (x::k); subst; split; simpl; auto.
+               apply merge_sorted with (1 := H3) (5 := G1); auto.
+          - refine (let (k,G) := IH l m' _ _ _ in _); auto; try destruct G as (G1 & G2).
+            ++ subst; simpl; omega.
+            ++ revert Hm; subst; apply sorted_inv_sorted.
+            ++ exists (y::k); subst; split; auto.
+               apply merge_sorted with (1 := H3) (2 := Hm) (3 := Hl); auto.
+               apply perm_trans with (1 := G1), 
+                     perm_trans with (2 := perm_middle _ _ _ _),
+                     perm_cons, perm_app_comm.
+    Defined.
+
+  End merge.
+
+  Fixpoint halve m : list nat * list nat :=
+    match m with
+      | nil      => (nil,nil)
+      | x::nil   => (m,nil)
+      | x::y::m' => let (l',r') := halve m' in (x::l',y::r')
+    end. 
+
+  Fact halve_spec m : let (l,r) := halve m 
+                      in m ~p l++r 
+                      /\ length r <= length l <= 1 + length r. 
+  Proof.
+    induction m as [ [ | x [ | y m ] ] IH ] using (measure_rect _ (@length _)); simpl.
+    + split; auto; constructor.
+    + split; auto; repeat constructor.
+    + specialize (IH m).
+      destruct (halve m).
+      destruct IH; simpl; auto; split; auto; omega.
+  Qed.
+
+  Definition merge_sort m : { k | m ~p k /\ sorted k }.
+  Proof.
+    induction m as [ m IH ] using (measure_rect _ (@length _)).
+    generalize (halve_spec m).
+    refine (match halve m with (l,r) => _ end); intros (H1 & H2).
+    case_eq r.
+    + intros H3; exists l; split.
+      * subst; rewrite <- app_nil_end in H1; auto.
+      * destruct l as [ | x [ | y l ] ]; auto.
+        subst; simpl in H2; omega.
+    + intros y r' Hr.
+      refine (let (l',G1) := IH l _ in
+              let (r',G3) := IH r _ in _).
+      * apply perm_length in H1; simpl; subst.
+        rewrite H1, app_length; simpl; omega.
+      * apply perm_length in H1; simpl; subst.
+        rewrite H1, app_length; simpl in H2; omega.
+      * destruct G1 as (G1 & G2).
+        destruct G3 as (G3 & G4).
+        refine (let (k,G) := merge l' r' G2 G4 in _).
+        destruct G as (G5 & G6).
+        exists k; split; auto.
+        apply perm_trans with (1 := H1), perm_sym,
+              perm_trans with (1 := G5), perm_sym; auto.
+  Defined.
+
+End mergesort.
+
+Recursive Extraction merge_sort.
